test/ctypes/Lowlevel.fst
@@ -2,24 +2,26 @@ module Lowlevel
 
 (** Dummy types and functions for testing the -ctypes option *)
 
+open FStar.Mul
+open FStar.UInt
 open FStar.HyperStack.ST
 
 module B = LowStar.Buffer
 module M = LowStar.Modifies
 module U32 = FStar.UInt32
 
+
 type point = { x: U32.t; y: U32.t }
 type circle = { c: point; r: U32.t }
 
 let square (x: U32.t): U32.t =
-
-  let open FStar.UInt32 in
+  let open U32 in
   x *%^ x
 
 val point_sum: p1: point -> p2: point -> Stack point
   (requires fun h ->
-    U32.v p1.x + U32.v p2.x < 32 /\
-    U32.v p1.y + U32.v p2.y < 32)
+    size (U32.v p1.x + U32.v p2.x) U32.n /\
+    size (U32.v p1.y + U32.v p2.y) U32.n)
   (ensures fun h0 _ h1 -> True)
 let point_sum p1 p2 =
   let open FStar.UInt32 in
@@ -28,8 +30,8 @@ let point_sum p1 p2 =
 
 val move_circle: cir: circle -> d: point -> Stack circle
   (requires fun h ->
-    U32.v cir.c.x + U32.v d.x < 32 /\
-    U32.v cir.c.y + U32.v d.y < 32)
+    size (U32.v cir.c.x + U32.v d.x) U32.n /\
+    size (U32.v cir.c.y + U32.v d.y) U32.n)
   (requires fun h0 _ h1 -> True)
 let move_circle cir d =
   let open FStar.UInt32 in
@@ -50,29 +52,41 @@ let my_not b =
   ()
 
 // Inductives: record compilation scheme
-type tr = | Rec of U32.t * U32.t * U32.t * U32.t * U32.t
-val replicate: n: U32.t -> Stack tr
-  (requires fun h -> True)
-  (requires fun h0 _ h1 -> True)
+type tr = | Rec of U32.t & U32.t & U32.t & U32.t & U32.t
+val replicate: n: U32.t -> St tr
 let replicate n =
   Rec (n, n, n, n, n)
 
+// Inductives: optimised flat compilation scheme
+type int_opt = | IntSome of U32.t | IntNone
+val maybe_double: opt: B.pointer int_opt -> Stack unit
+  (requires fun h -> B.live h opt /\
+     (match FStar.Seq.Base.index (B.as_seq h opt) 0 with
+     | IntSome n -> size (2 * U32.v n) U32.n
+     | IntNone -> True))
+  (requires fun h0 _ h1 -> True)
+let maybe_double opt =
+  let open U32 in
+  let open LowStar.Monotonic.Buffer in
+  let v = match B.index opt 0ul with
+    | IntSome d -> IntSome (2ul *^ d)
+    | IntNone -> IntNone
+  in
+  upd opt 0ul v
 
-// // Inductives: optimised flat compilation scheme
-// type int_opt = | Some of U32.t | None
+val gen_adder: U32.t -> St (U32.t -> U32.t)
+let gen_adder a =
+  let open U32 in
+  (fun x -> a +%^ x)
+
+
+// Not supported:
 
 // // Inductives: general compilation scheme
-// assume new type foo
-// assume new type bar
-// noeq type t_general = | A of foo | B of bar
-
-
-// val my_not: b: B.pointer U32.t -> Stack unit
-//   (requires fun h -> B.live h b)
-//   (requires fun h0 _ h1 -> B.live h1 b)
-// let my_not b =
-//   let open LowStar.Monotonic.Buffer in
-//   let v = B.index b 0ul in
-//   upd b 0ul 5ul;
-//   ()
+// noeq type eith = | L of U32.t | R of U32.t
+// val flip_t: x: eith -> St eith
+// let flip_t x =
+//   match x with
+//   | L n -> R n
+//   | R n -> L n
 
